Fp/SmtLibSemantics.lean
@@ -8,6 +8,7 @@ open Lean
 
 namespace Fp
 namespace SmtLibSemantics
+
 /-
 We follow the development from
 "An Automatable Formal Semantics for IEEE-754 Floating-Point Arithmetic" [1]
@@ -34,9 +35,36 @@ def ExtendedNumber.ltZero {R : Type} [ExtendedNumber R] (r : R) : Prop :=
 def ExtendedNumber.gtZero {R : Type} [ExtendedNumber R] (r : R) : Prop :=
   (Zero.zero) < r
 
-instance : ExtendedNumber ExtRat where
+instance [hEx : ExtendedNumber R] [DecidableRel ((· < ·) : R → R → Prop)] :
+    DecidablePred (hEx.ltZero : R → Prop) := by
+  unfold ExtendedNumber.ltZero
+  infer_instance
+instance [hEx : ExtendedNumber R] [DecidableRel ((· < ·) : R → R → Prop)] :
+    DecidablePred (hEx.gtZero : R → Prop) := by
+  unfold ExtendedNumber.gtZero
+  infer_instance
+
+instance [hEx : ExtendedNumber R] [DecidableRel hEx.extendedEq] :
+    DecidablePred hEx.isZero := by
+  unfold ExtendedNumber.isZero
+  infer_instance
+
+
+instance instExtendedRat : ExtendedNumber ExtRat where
   isNaN r := r.isNaN
   extendedEq r1 r2 := r1.eq r2
+
+instance : Decidable (instExtendedRat.isZero r) := by
+  simp [ExtendedNumber.isZero, ExtendedNumber.extendedEq]
+  infer_instance
+
+instance : Decidable (instExtendedRat.isNaN r) := by
+  simp [ExtendedNumber.isNaN]
+  infer_instance
+
+instance : DecidableRel instExtendedRat.extendedEq := by
+  simp [ExtendedNumber.extendedEq]
+  infer_instance
 
 /-- Embed the type `X` into the extended rationals. -/
 class RoundableEmbed (X : Type) (R : Type) where
@@ -99,12 +127,13 @@ structure RoundablePredicates (X : Type) (R : Type) extends
   RoundableIsEven X
   where
 
-
 structure RoundMethod (X : Type) (R : Type) extends
   RoundableAdjunction X R,
   RoundablePredicates X R
 
-def RoundMethod.rounderForSign {X : Type} (roundMethod : RoundMethod X R) (sign : Bool) (r : R) : X :=
+def RoundMethod.rounderForSign {X : Type}
+    (roundMethod : RoundMethod X R)
+    (sign : Bool) (r : R) : X :=
   if sign then roundMethod.upper r else roundMethod.lower r
 
 open  ExtendedNumber in
@@ -121,17 +150,17 @@ def RoundMethod.round {e s R} (roundMethod : RoundMethod (PackedFloat e s) R) [i
   | .RNE =>
       if isNaN r then roundMethod.lower r
       else if isZero r then roundMethod.rounderForSign sign r
-      else if ¬ (isZero r) ∧ roundMethod.lowerHalf r then roundMethod.lower r
-      else if ¬ (isZero r) ∧ roundMethod.tieBreak r ∧ roundMethod.isEven (roundMethod.lower r) then roundMethod.lower r
-      else if ¬ (isZero r) ∧ roundMethod.tieBreak r ∧ roundMethod.isEven (roundMethod.upper r) then roundMethod.upper r
-      else if ¬ (isZero r) ∧ ¬ roundMethod.lowerHalf r ∧ ¬ roundMethod.tieBreak r then roundMethod.upper r
+      else if ! decide (isZero r) && roundMethod.lowerHalf r then roundMethod.lower r
+      else if ! decide (isZero r) && roundMethod.tieBreak r && roundMethod.isEven (roundMethod.lower r) then roundMethod.lower r
+      else if ! decide (isZero r) && roundMethod.tieBreak r && roundMethod.isEven (roundMethod.upper r) then roundMethod.upper r
+      else if ! decide (isZero r) && !roundMethod.lowerHalf r && !roundMethod.tieBreak r then roundMethod.upper r
       else .mkNaN -- does not occur.
   | .RNA =>
-      if gtZero r ∧ ¬ (roundMethod.lowerHalf r) then roundMethod.upper r
-      else if gtZero r ∧ (roundMethod.lowerHalf r) then roundMethod.lower r
+      if gtZero r && !(roundMethod.lowerHalf r) then roundMethod.upper r
+      else if gtZero r && (roundMethod.lowerHalf r) then roundMethod.lower r
       else if isZero r then roundMethod.rounderForSign sign r
       else if isNaN r then roundMethod.lower r
-      else if ltZero r ∧ ¬ (roundMethod.lowerHalf r) ∧ ¬ (roundMethod.tieBreak r) then roundMethod.upper r
+      else if ltZero r && ! (roundMethod.lowerHalf r) && ! (roundMethod.tieBreak r) then roundMethod.upper r
       else if ltZero r && (roundMethod.lowerHalf r) || (roundMethod.tieBreak r) then roundMethod.lower r
       else .mkNaN -- does not occur.
    | .RTP =>
@@ -197,7 +226,7 @@ def smtLibRoundMethod (e s : Nat)
   embed := v.embed
   lower := v.lower
   upper := v.upper
-  lowerHalf r := v.embed (v.lower r) = ves.embed (ves.lower r)
+  lowerHalf r := ExtendedNumber.extendedEq (v.embed (v.lower r))  (ves.embed (ves.lower r))
   /-
   The SMT-LIb specification would have one write:
   ```lean
@@ -216,6 +245,25 @@ def smtLibRoundMethod (e s : Nat)
     (v.embed (v.lower r) < ves.embed (ves.lower r)) =
     (ves.embed (ves.upper r) < (v.embed (v.upper r)))
   isEven := roundableIsEven_of_packedFloat.isEven
+
+instance [hExtended : ExtendedNumber R]
+    [DecidableRel hExtended.extendedEq]
+    {v : RoundableAdjunction (PackedFloat e s) R}
+    {ves : RoundableAdjunction (PackedFloat e (s + 1)) R} :
+    DecidablePred ((smtLibRoundMethod e s v ves).lowerHalf) := by
+  simp [smtLibRoundMethod]
+  infer_instance
+
+set_option trace.Meta.synthInstance true in
+instance [hExtended : ExtendedNumber R]
+    [hdec : ((r s : R) → Decidable (r < s))]
+    {v : RoundableAdjunction (PackedFloat e s) R}
+    {ves : RoundableAdjunction (PackedFloat e (s + 1)) R} :
+    DecidablePred ((smtLibRoundMethod e s v ves).tieBreak) := by
+  simp [smtLibRoundMethod]
+  infer_instance
+
+  -- infer_instance
 
 end SmtLibRoundMethod
 
