Fp/Tests/SmtLibSemanticsComputable.lean
@@ -1,0 +1,143 @@
+import Fp.Rounding
+import Fp.SmtLibSemantics
+
+namespace Fp
+open SmtLibSemantics
+
+namespace SmtLibSemanticsComputable
+
+structure PackedFloatEnumeration (e : Nat) (s : Nat) where ofEnumeration ::
+  -- | Sorted array of packed float with its rational value. Only numbers,
+  -- no infinities and NaNs.
+  enumeration : Array (PackedFloat e s × Rat)
+
+
+def PackedFloatEnumeration.mk (e s : Nat) : PackedFloatEnumeration e s where
+  enumeration := Id.run do
+    let mut arr : Array (PackedFloat e s × Rat) := #[]
+    for sign in [true, false] do
+      for exp in [:2^e] do
+        for sig in [:2^s] do
+          let pf : PackedFloat e s := PackedFloat.mk sign exp sig
+          let er := pf.toExtRat
+          let ExtRat.Number r := er
+            | continue
+          arr := arr.push (pf, r)
+    arr.qsort (fun (_, r1) (_, r2) => r1 < r2)
+
+def PackedFloatEnumeration.minNumber (enum : PackedFloatEnumeration e s) : PackedFloat e s × Rat :=
+  enum.enumeration[0]!
+
+def PackedFloatEnumeration.maxNumber (enum : PackedFloatEnumeration e s) : PackedFloat e s × Rat :=
+  enum.enumeration[enum.enumeration.size - 1]!
+
+def PackedFloatEnumeration.greatestLowerBound (enum : PackedFloatEnumeration e s)
+    (r : Rat) : Option (PackedFloat e s × Rat) := Id.run do
+  let arr := enum.enumeration
+  let mut glb? := none
+  for hi : i in [:arr.size] do
+    let (curPf, curRat) := arr[i]
+    if curRat <= r then
+        -- is a lower bound
+        glb? :=
+          match glb? with
+          | none => some (curPf, curRat)
+          | some (_, glbRat) =>
+            -- is larger than the current lower bound.
+            if curRat > glbRat then
+              some (curPf, curRat)
+            else
+              glb?
+  glb?
+
+def PackedFloatEnumeration.leastUpperBound (
+    enum : PackedFloatEnumeration e s)
+    (r : Rat) : Option (PackedFloat e s × Rat) := Id.run do
+  let arr := enum.enumeration
+  let mut lub? := none
+  for hi : i in [0:arr.size] do
+    let (curPf, curRat) := arr[i]
+    if curRat >= r then
+        -- is an upper bound
+        lub? :=
+          match lub? with
+          | none => some (curPf, curRat)
+          | some (_, lubRat) =>
+            -- is smaller than the current upper bound.
+            if curRat < lubRat then
+              some (curPf, curRat)
+            else
+              lub?
+  lub?
+
+def mkZero (sign : Bool) (e s : Nat) : PackedFloat e s :=
+  EUnpackedFloat.mkNumber (UnpackedFloat.mkZero sign) |>.pack
+
+
+/-
+This file defines a computable version of the SMT-LIB semantics,
+which is used for comparing results from SMT solvers with those from Lean's floating-point library.
+-/
+
+def lowerFromEmbedByEnumeration {e s}
+    (enum : PackedFloatEnumeration e s) :
+    RoundableLower (PackedFloat e s) ExtRat where
+  lower := fun (r : ExtRat) =>
+    match r with
+    | .NaN => .mkNaN
+    | .Infinity x => .getInfinity e s x -- infinity is representable.
+    | .Number r =>
+      -- for a number, if it is below the min number, return -inf
+      match enum.greatestLowerBound r with
+      | some (pf, rpf) =>
+        if rpf = 0
+        then mkZero false e s -- lower bound is +0 (footnote 5)
+        else pf
+      | none => PackedFloat.getInfinity _ _ true
+
+
+def upperFromEmbedByEnumeration {e s}
+    (enum : PackedFloatEnumeration e s) :
+    RoundableUpper (PackedFloat e s) ExtRat where
+  upper := fun (r : ExtRat) =>
+    match r with
+    | .NaN => .mkNaN
+    | .Infinity x => .getInfinity e s x -- infinity is representable.
+    | .Number r =>
+      -- for a number, if it is above the max number, return +inf
+      match enum.leastUpperBound r with
+      | some (pf, rpf) =>
+          if rpf = 0
+          then mkZero true e s -- upper bound is -0 (footnote 5)
+          else pf
+      | none => PackedFloat.getInfinity _ _ false
+
+def computableV : RoundableAdjunction (PackedFloat e s) ExtRat where
+  lower := lowerFromEmbedByEnumeration (PackedFloatEnumeration.mk e s) |>.lower
+  upper := upperFromEmbedByEnumeration (PackedFloatEnumeration.mk e s) |>.upper
+  embed := PackedFloat.toExtRat
+
+abbrev computableSmtLibRoundMethod (e s : Nat) :
+    RoundMethod (PackedFloat e s) ExtRat :=
+  SmtLibRoundMethod.smtLibRoundMethod e s
+    (computableV)
+    (computableV)
+
+instance : DecidablePred ((computableSmtLibRoundMethod e s).lowerHalf) := by
+  simp [computableSmtLibRoundMethod]
+  infer_instance
+
+instance : DecidablePred ((computableSmtLibRoundMethod e s).tieBreak) := by
+  simp [computableSmtLibRoundMethod]
+  infer_instance
+
+
+/-- A computable version of the SMT-LIB rounder functions. -/
+def computableSmtLibRound {e s : Nat}
+  (rm : RoundingMode) (sign : Bool)
+  (r : ExtRat) : PackedFloat e s :=
+  (computableSmtLibRoundMethod e s).round rm sign r
+
+end SmtLibSemanticsComputable
+
+end Fp
